Start trying to prove installed for hello_ag32

examples/ag32/compilation/proofs/hello_ag32ProofScript.sml
@@ -11,6 +11,155 @@ val hello_outputs_def =
 val (hello_sem,hello_output) = hello_outputs_def |> CONJ_PAIR
 val (hello_not_fail,hello_sem_sing) = MATCH_MP semantics_prog_Terminate_not_Fail hello_sem |> CONJ_PAIR
 
+val ffi_names =
+  ``config.ffi_names``
+  |> (REWRITE_CONV[hello_ag32CompileTheory.config_def] THENC EVAL)
+
+val hello_machine_config_def = Define`
+  hello_machine_config r0 = <|
+    target := ag32_target;
+    ptr_reg := 1;
+    len_reg := 2;
+    ptr2_reg := 3;
+    len2_reg := 4;
+    callee_saved_regs := [60; 61; 62];
+    ffi_names := ^(rand(rconc ffi_names));
+    ffi_entry_pcs := [r0 + 64w];
+    ccache_pc := r0 + 64w +  n2w ffi_offset;
+    halt_pc := r0 + 64w + n2w (2 * ffi_offset) ;
+    prog_addresses := { w | r0 + 64w + n2w (3 * ffi_offset) <=+ w ∧ w <+ r0 + (n2w (128 * 2 ** 10)) }
+  |>`
+
+val is_ag32_machine_config_hello_machine_config = Q.store_thm("is_ag32_machine_config_hello_machine_config",
+  `is_ag32_machine_config (hello_machine_config r0)`, EVAL_TAC);
+
+val hello_init_memory_def = Define`
+  hello_init_memory (k:word32) = (0w:word8)`;
+
+val hello_init_regs_def = Define`
+  hello_init_regs (k:num) = (0w:word32)`;
+
+val hello_init_ag32_state_def = Define`
+  hello_init_ag32_state (r0:word32) = <|
+    PC := r0 + 64w + n2w (3 * ffi_offset) ;
+    MEM := hello_init_memory ;
+    R := hello_init_regs o w2n
+  |>`;
+
+val hello_init_asm_state_def = Define`
+  hello_init_asm_state (r0:word32) = <|
+    be := F;
+    lr := 0 ;
+    failed := F ;
+    align := 2 ;
+    pc := r0 + 64w + n2w (3 * ffi_offset);
+    mem := hello_init_memory ;
+    mem_domain := (hello_machine_config r0).prog_addresses ;
+    regs := hello_init_regs
+  |>`;
+
+val hello_good_init_state = Q.store_thm("hello_good_init_state",
+  `aligned 2 r0 ⇒
+   good_init_state (hello_machine_config r0) (hello_init_ag32_state r0)
+     ag_ffi code 0 (hello_init_asm_state r0) m
+       ({w | (hello_init_asm_state r0).regs 2 <=+ w ∧ w <+ (hello_init_asm_state r0).regs 4}
+        ∪ bitmaps_dm) io_regs cc_regs`,
+  strip_tac
+  \\ simp[lab_to_targetProofTheory.good_init_state_def]
+  \\ conj_tac
+  >- (
+    simp[asmPropsTheory.target_state_rel_def]
+    \\ simp[EVAL``(hello_machine_config r0).target``]
+    \\ conj_tac
+    >- (
+      simp[ag32_targetTheory.ag32_ok_def, hello_init_ag32_state_def]
+      \\ (alignmentTheory.aligned_add_sub_cor
+          |> SPEC_ALL |> UNDISCH |> CONJUNCT1 |> DISCH_ALL
+          |> irule)
+      \\ reverse conj_tac >- EVAL_TAC
+      \\ (alignmentTheory.aligned_add_sub_cor
+          |> SPEC_ALL |> UNDISCH |> CONJUNCT1 |> DISCH_ALL
+          |> irule)
+      \\ reverse conj_tac >- EVAL_TAC
+      \\ fs[] )
+    \\ conj_tac >- EVAL_TAC
+    \\ conj_tac >- (EVAL_TAC \\ rw[])
+    \\ EVAL_TAC \\ rw[] )
+  \\ conj_tac
+  >- (
+    simp[lab_to_targetProofTheory.target_configured_def]
+    \\ conj_tac >- EVAL_TAC
+    \\ simp[EVAL``(hello_machine_config r0).target``]
+    \\ simp[hello_init_asm_state_def]
+    \\ once_rewrite_tac[WORD_AND_COMM]
+    \\ Cases
+    \\ rewrite_tac[word_add_n2w]
+    \\ rewrite_tac[addressTheory.n2w_and_3]
+    \\ qx_gen_tac`m`
+    \\ cheat (* target_configured needs to be fixed *) )
+  \\ conj_tac >- EVAL_TAC
+  \\ `r0 + 64w + 48w && 3w = 0w` by (
+    fs[alignmentTheory.aligned_bitwise_and]
+    \\ Cases_on`r0`
+    \\ simp[word_add_n2w]
+    \\ once_rewrite_tac[WORD_AND_COMM]
+    \\ rewrite_tac[addressTheory.n2w_and_3]
+    \\ qpat_x_assum`_ = 0w`mp_tac
+    \\ once_rewrite_tac[WORD_AND_COMM]
+    \\ rewrite_tac[addressTheory.n2w_and_3]
+    \\ simp[] )
+  \\ `r0 + 64w + 48w && 1w = 0w` by (
+    fs[alignmentTheory.aligned_bitwise_and]
+    \\ Cases_on`r0`
+    \\ simp[word_add_n2w]
+    \\ once_rewrite_tac[WORD_AND_COMM]
+    \\ rewrite_tac[addressTheory.n2w_and_1]
+    \\ qpat_x_assum`_ && n2w n = 0w`mp_tac
+    \\ once_rewrite_tac[WORD_AND_COMM]
+    \\ rewrite_tac[addressTheory.n2w_and_3]
+    \\ simp[]
+    \\ DEP_ONCE_REWRITE_TAC[LESS_MOD]
+    \\ conj_tac
+    >- (
+      match_mp_tac LESS_LESS_EQ_TRANS
+      \\ qexists_tac`4`
+      \\ simp[MOD_LESS] )
+    \\ strip_tac
+    \\ DEP_ONCE_REWRITE_TAC[LESS_MOD]
+    \\ conj_tac
+    >- (
+      match_mp_tac LESS_LESS_EQ_TRANS
+      \\ qexists_tac`2`
+      \\ simp[MOD_LESS] )
+    \\ fs[MOD_EQ_0_DIVISOR]
+    \\ qexists_tac`2 * d`
+    \\ simp[] )
+  \\ conj_tac
+  >- (
+    rewrite_tac[lab_to_targetProofTheory.start_pc_ok_def]
+    \\ conj_tac >- cheat (* word proof, may need to tweak prog_addresses? or add assums? *)
+    \\ conj_tac >- cheat (* word proof, may need to tweak prog_addresses? or add assums? *)
+    \\ conj_tac >- (EVAL_TAC \\ simp[])
+    \\ conj_tac >- (EVAL_TAC \\ simp[])
+    \\ conj_tac >- ( EVAL_TAC \\ fs[] )
+    \\ rewrite_tac[EVAL``(hello_machine_config r0).ffi_names``]
+    \\ reverse Cases >- rw[]
+    \\ strip_tac
+    \\ conj_tac >- cheat (* word proof, may need to tweak prog_addresses? or add assums? *)
+    \\ conj_tac >- cheat (* word proof, may need to tweak prog_addresses? or add assums? *)
+    \\ conj_tac >- cheat (* word proof, may need to tweak prog_addresses? or add assums? *)
+    \\ EVAL_TAC \\ rw[] )
+  \\ conj_tac >- ( EVAL_TAC \\ fs[] )
+  \\ conj_tac >- (
+    rw[asmPropsTheory.interference_ok_def]
+    \\ simp[EVAL``(hello_machine_config r0).target``]
+    \\ cheat (* set next_interfer to identity function? *) )
+  \\ conj_tac >- cheat (* ffi - set ffi_interfer based on hello outputs and some function modeling the print call? *)
+  \\ conj_tac >- cheat (* set ccache_interfer to identity function? *)
+  \\ conj_tac >- cheat (* set hello_init_memory to contain the code at the right pc *)
+  \\ conj_tac >- cheat (* code in memory again? *)
+  \\ cheat);
+
 val compile_correct_applied =
   MATCH_MP compile_correct hello_compiled
   |> SIMP_RULE(srw_ss())[LET_THM,ml_progTheory.init_state_env_thm,GSYM AND_IMP_INTRO]
@@ -20,11 +169,16 @@ val compile_correct_applied =
   |> REWRITE_RULE[Once (GSYM AND_IMP_INTRO)]
   |> C MATCH_MP (CONJ(UNDISCH ag32_machine_config_ok)(UNDISCH ag32_init_ok))
   |> DISCH(#1(dest_imp(concl ag32_init_ok)))
-  |> REWRITE_RULE[AND_IMP_INTRO]
+  |> C MATCH_MP is_ag32_machine_config_hello_machine_config
+  |> Q.GEN`cbspace` |> Q.SPEC`0`
+  |> Q.GEN`data_sp` |> Q.SPEC`0`
+  |> Q.GEN`ms` |> SPEC(lhs(concl(SPEC_ALL hello_init_ag32_state)))
 
-val hello_compiled_thm =
-  CONJ compile_correct_applied hello_output
-  |> DISCH_ALL
-  |> curry save_thm "hello_compiled_thm";
+(*
+val goal = compile_correct_applied |> concl |> dest_imp |> #1
+set_goal([],goal)
+CONV_TAC(PATH_CONV"llr"EVAL)
+\\ rw[backendProofTheory.installed_def]
+*)
 
 val _ = export_theory();
